@prefix :       <http://purl.org/semwiq/mediator/sdv#> .
@prefix rdf:    <http://www.w3.org/1999/02/22-rdf-syntax-ns#> .
@prefix rdfs:   <http://www.w3.org/2000/01/rdf-schema#> .
@prefix xsd:    <http://www.w3.org/2001/XMLSchema#> .
@prefix owl:	<http://www.w3.org/2002/07/owl#> .
@prefix foaf:   <http://xmlns.com/foaf/0.1/> .
@prefix rsc:	<http://purl.org/rdfstats/configuration#> .
@prefix void:	<http://rdfs.org/ns/void#> .

:required					a rdf:Property ;
	rdfs:label				"required" ;
	rdfs:comment			"indicates that a property or instance of some class is required for a catalog to be valid" ;
	rdfs:domain				rdfs:Resource ;
	rdfs:range				xsd:boolean .

<>	rdfs:label "SemWIQ DataSource Vocabulary" ;
	rdfs:comment "Describes data sources registered at a SemWIQ mediator node. When there is a first stable version of voiD (see http://community.linkeddata.org/MediaWiki/index.php?VoiD), this vocabulary will be migrated or at least linked to voiD."
	.

:lastDownload		a rdf:Property ;
	rdfs:label		"last download" ;
	rdfs:comment	"allows to mark resources with a timestamp to indicate when they were downloaded from the Web into the global store (e.g. used for RDFStatsDataset)" ;
	rdfs:domain		rdfs:Resource ;
	rdfs:range		xsd:dateTime .
	

##### Extensions to voiD #####

:DataSource		a owl:Class ;
	rdfs:label "SPARQL data source" ;
	rdfs:comment "data source accessible via the SPARQL protocol - Instead of introducing a new data source vocabulary, we assume that each void:Dataset that has a void:sparqlEndpoint property is a valid data source" ;
	rdfs:subClassOf void:Dataset ;
	rdfs:subClassOf [
		a owl:Restriction ;
		owl:onProperty void:sparqlEndpoint ;
		owl:cardinality "1"^^xsd:nonNegativeInteger ;
	] .

:disabled
      a       rdf:Property ;
      rdfs:comment "allows to explicitly specify that a data source is disabled" ;
      rdfs:domain :DataSource ;
      rdfs:range xsd:boolean .

:unavailable
      a       rdf:Property ;
      rdfs:comment "this property is used internally by SemWIQ to mark data sources as temporarily unavailable, it will be added/changed by the data source monitor" ;
      rdfs:domain :DataSource ;
      rdfs:range xsd:boolean .

:subsumption
	a rdf:Property ;
	rdfs:comment "specifies that the data source is capable of subsumption reasoning itself, default is false" ;
	rdfs:domain :DataSource ;
	rdfs:range xsd:boolean .
	
:monitoringProfile
      a       rdf:Property ;
      rdfs:comment "specific data source monitor options, if omitted the data source is monitored by the default :VoidMonitoringProfile" ;
      rdfs:domain :DataSource ;
      rdfs:range :MonitoringProfile .


##### MonitoringOptions #####

:MonitoringProfile
	a rdfs:Class ;
	rdfs:comment "abstract class - specifies monitoring options and can be applied for multiple data sources" .

:interval
	a rdf:Property ;
	rdfs:comment "interval for update request in seconds" ;
	rdfs:domain :MonitoringProfile ;
	rdfs:range xsd:int ;
	.

:updateOnStartup
	a rdf:Property ;
	rdfs:comment "" ;
	rdfs:domain :MonitoringProfile ;
	rdfs:range xsd:boolean ;
	.
	

##### centralized

:CentralizedMonitoringProfile
	a rdfs:Class ;
	rdfs:subClassOf :MonitoringProfile ;
	rdfs:comment "defines centralized monitoring and specifies monitoring options" .

:statsConfig
	a rdf:Property ;
	rdfs:comment "overrides global RDFStats configuration (ignoring explicit properties rsc:endpoint, rsc:statsModel, rsc:outputFile, and rsc:outputFormat)" ;
	rdfs:domain :CentralizedMonitoringProfile ;
	rdfs:range rsc:RDFStatsConfiguration .


##### remote

:RemoteMonitoringProfile
	a rdfs:Class ;
	rdfs:subClassOf :MonitoringProfile ;
	rdfs:comment "defines remote monitoring (RDFStats installed at end-point) and specifies monitoring options" .

:statsUrl
	a rdf:Property ;
	rdfs:comment """Optional custom URL from where to retrieve RDFStats statistics. The default is '%%PROTOCOL%%://%%DOMAIN%%:%%PORT%%/rdfstats-%%PORT%%.nt.zip'.
The following macros can be used and will be replaced by the corresponding values of a concrete data source's SPARQL endpoint URI. 
%%ENDPOINT-URI%%, %%PROTOCOL%%, %%DOMAIN%%, %%PORT%%, %%PATH%%.""" ;
	rdfs:domain :RemoteMonitoringProfile ;
	rdfs:range rdfs:Resource .

###### void profile

:VoidMonitoringProfile
	a rdfs:Class ;
	rdfs:subClassOf :MonitoringProfile ;
	rdfs:comment "monitors data sources by retrieving voiD metadata according to robots.txt. => sitemap.xml => void:Dataset in RDF" .

:updateOnlyIfNewer
	a rdf:Property ;
	rdfs:comment "update dataset only if remote statistics are newer" ;
	rdfs:domain :RemoteMonitoringProfile , :VoidMonitoringProfile ;
	rdfs:range xsd:boolean ;
	.

